src/compare.v
@@ -1,0 +1,77 @@
+From stdpp Require Import base.
+From marble Require Import tactics wp wp_tactics orders sorting.
+
+Unset Universe Minimization ToSet.
+Generalizable All Variables.
+Set Universe Polymorphism.
+
+(* -------------------------------------------------------------------------- *)
+
+(* Three-way comparisons. *)
+
+(* This type exists in the standard library:
+Inductive comparison := Eq | Lt | Gt.
+ *)
+
+(* A [compare] function performs a three-way comparison. *)
+
+(* [Compare A] means that the type [A] has a [compare] function. *)
+
+Class Compare (A : Type) :=
+  { compare : A → A → comparison }.
+
+(* [Comparable A] means that the [compare] function at type [A]
+   is correct with respect to the default preorder on this type. *)
+
+Section Comparable.
+
+Open Scope element_scope.
+
+Context (A : Type) (R : relation A).
+
+(* Standard mathematical notation. *)
+
+Infix "≤" := R
+  (at level 70, no associativity) : element_scope.
+Infix "<" := (strict R)
+  (at level 70, no associativity) : element_scope.
+Notation "y ≥ x" := (x ≤ y)
+  (only parsing, at level 70, no associativity) : element_scope.
+Notation "y > x" := (x < y)
+  (only parsing, at level 70, no associativity) : element_scope.
+Infix "≡" := (equivalent R)
+  (at level 70, no associativity) : element_scope.
+
+(* Standard mathematical facts about the above definitions. *)
+
+Lemma equiv_le x y :  x ≡ y → x ≤ y.
+Proof. unfold equivalent. tauto. Qed.
+Lemma lt_le x y :  x < y → x ≤ y.
+Proof. unfold strict. tauto. Qed.
+Lemma equiv_ge x y :  x ≡ y → x ≥ y.
+Proof. unfold equivalent. tauto. Qed.
+Lemma gt_ge x y :  x > y → x ≥ y.
+Proof. eauto using lt_le. Qed.
+
+Context `{Compare A}.
+
+Class Comparable := {
+  compare_spec :
+    ∀ x y : A, CompareSpec (x ≡ y) (x < y) (x > y) (compare x y)
+}.
+
+Lemma wp_compare_Gt_Le `{Comparable} {B} (x y : A) (e1 e2 : B) (Q : B → Prop) :
+  (x > y → wp e1 Q) →
+  (x ≤ y → wp e2 Q) →
+  wp (match compare x y with Gt => e1 | _ => e2 end) Q.
+Proof.
+  intros. destruct (compare_spec x y).
+  + eauto using equiv_le.
+  + eauto using lt_le.
+  + eauto.
+Qed.
+
+End Comparable.
+
+Global Ltac wp_compare :=
+  simple eapply wp_compare_Gt_Le; [ eauto | intro | intro ].
